

# **CSE215**

# **Foundations of Computer Science**

**Instructor: Zhoulai Fu**

**State University of New York, Korea**

**April 13, 2022**

# Agenda

- Final exercises on mathematical induction

**Finish around 4h45**

# 2020 Midterm-2

**Problem 1. [20 points]**

Use mathematical induction to prove the following identities.

(a) [5 points] For integers  $n \geq 1$ ,

$$\sum_{i=1}^n \frac{1}{(2i-1)(2i+1)} = \frac{n}{2n+1}$$

(b) [5 points] For integers  $n \geq 1$ ,

$$1^2 - 2^2 + 3^2 - \cdots + (-1)^{n-1}n^2 = (-1)^{n-1} \frac{n(n+1)}{2}$$

(c) [5 points]  $9^n + 3$  is divisible by 4 for integers  $n \geq 1$ .

(d) [5 points] Suppose that  $g_1, g_2, g_3, \dots$  is a sequence defined as follows:

$$g_1 = 3, g_2 = 5$$

$$g_k = 3g_{k-1} - 2g_{k-2} \quad \text{for all integers } k \geq 3.$$

Prove that  $g_n = 2^n + 1$  for all integers  $n \geq 1$ .

(a) [5 points] For integers  $n \geq 1$ ,

$$\sum_{i=1}^n \frac{1}{(2i-1)(2i+1)} = \frac{n}{2n+1}$$

- Proof.
  - Let  $P(n)$  be the predicate  $1/(1*3) + 1/(3*5) + \dots 1/((2n-1)(2n+1)) = n/(2n+1)$
  - Base step: We prove  $P(1)$ .
  - Inductive step: We prove for any integer  $k \geq 1$ ,  $P(k) \rightarrow P(k+1)$ 
    - Let  $k$  be an arbitrary integer and  $k \geq 1$ .
    - Assume  $P(k)$  holds. That is  $1/(1*3) + 1/(3*5) + \dots 1/((2k-1)(2k+1)) = k/(2k+1)$
    - We need to prove  $P(k+1)$ , namely,  $1/(1*3) + 1/(3*5) + \dots 1/((2k-1)(2k+1)) + 1/((2k+1)(2k+3)) = (k+1)/(2k+3)$ 
      - Following assumption  $P(k)$ , LHS =  $k/(2k+1) + 1/((2k+1)(2k+3))$
      - $k/(2k+1) + 1/((2k+1)(2k+3)) = \dots = (k+1)/(2k+3)$
- QED.

(b) [5 points] For integers  $n \geq 1$ ,

$$1^2 - 2^2 + 3^2 - \cdots + (-1)^{n-1}n^2 = (-1)^{n-1} \frac{n(n+1)}{2}$$

- Proof.

- Let  $P(n)$  be the predicate  $1 + (-1)^2 \cdot 2^2 + \cdots + (-1)^n \cdot n^2 = (-1)^{n-1} \cdot n(n+1)/2$
- Base step: We prove  $P(1)$ .
- Inductive step: We prove for any integer  $k \geq 1$ ,  $P(k) \rightarrow P(k+1)$ 
  - Let  $k$  be an arbitrary integer and  $k \geq 1$ .
  - Assume  $P(k)$  holds. That is  $1 + \cdots + (-1)^k \cdot k^2 = (-1)^{k-1} \cdot k(k+1)/2$
  - We need to prove  $P(k+1)$ , namely,  $1 + \cdots + (-1)^k \cdot k^2 + (-1)^{k+1} \cdot (k+1)^2 = (-1)^k \cdot (k+1)(k+2)/2$ 
    - Following assumption  $P(k)$ ,  $\text{LHS} = (-1)^{k-1} \cdot k(k+1)/2 + (-1)^{k+1} \cdot (k+1)^2 = \dots = \text{RHS}$

- QED.

(c) [5 points]  $9^n + 3$  is divisible by 4 for integers  $n \geq 1$ .

- Proof.
  - Let  $P(n)$  be the predicate  $4|9^n+3$
  - Base step: We prove  $P(1)$  holds.
  - Inductive step: We prove for any integer  $k \geq 1$ ,  $P(k) \rightarrow P(k+1)$ 
    - Let  $k$  be an arbitrary integer and  $k \geq 1$ .
    - Assume  $P(k)$  holds  $4|9^k+3$ , namely  $9^k+3 = 4m$  for some integer  $m$ .
    - We need to prove  $P(k+1)$ , namely,  $4|9^{k+1}+3$ 
      - $9^{k+1}+3 = 9 * 9^k+3 = 9 * (9^k+3) - 24$
      - Following assumption  $P(k)$ ,  $9 * (9^k+3) - 24 = 36m - 24 = 4 * (9m - 6)$
- QED.

# 2021 Midterm-2

**Problem 1. [20 points]**

Use mathematical induction to prove the following identities.

(a) [5 points] For all integers  $n \geq 1$ ,

$$1 \cdot 2 \cdot 3 + 2 \cdot 3 \cdot 4 + \cdots + n(n+1)(n+2) = \frac{n(n+1)(n+2)(n+3)}{4}$$

(b) [5 points] For all integers  $n \geq 1$ ,  $n(n^2 + 5)$  is a multiple of 6.

(c) [5 points] For all integers  $n \geq 0$ ,

$$1 + \frac{2}{3} + \frac{4}{9} + \cdots + \left(\frac{2}{3}\right)^n = 3 \left[ 1 - \left(\frac{2}{3}\right)^{n+1} \right]$$

(d) [5 points] Suppose that  $c_1, c_2, c_3, \dots$  is a sequence defined as follows:

$$\begin{aligned} c_1 &= 3, c_2 = -9 \\ c_k &= 7c_{k-1} - 10c_{k-2} \quad \text{for all integers } k \geq 3 \end{aligned}$$

Prove that  $c_n = 4 \cdot 2^n - 5^n$  for all integers  $n \geq 1$ .

(a) [5 points] For all integers  $n \geq 1$ ,

$$1 \cdot 2 \cdot 3 + 2 \cdot 3 \cdot 4 + \cdots + n(n+1)(n+2) = \frac{n(n+1)(n+2)(n+3)}{4}$$

- Proof.
  - Let  $P(n)$  be the predicate  $1 \cdot 2 \cdot 3 + \cdots + n(n+1)(n+2) = n(n+1)(n+2)(n+3)/4$
  - Base step: We prove  $P(1)$  holds: LHS=6, RHS=6.
  - Inductive step: We prove for any integer  $k \geq 1$ ,  $P(k) \rightarrow P(k+1)$ 
    - Let  $k$  be an arbitrary integer and  $k \geq 1$ .
    - Assume  $P(k)$  holds. That is  $1 \cdot 2 \cdot 3 + \cdots + k(k+1)(k+2) = k(k+1)(k+2)(k+3)/4$
    - We need to prove  $P(k+1)$ , namely,  $1 \cdot 2 \cdot 3 + \cdots + k(k+1)(k+2) + (k+1)(k+2)(k+3) = (k+1)(k+2)(k+3)(k+4)/4$ 
      - LHS =  $k(k+1)(k+2)(k+3)/4 + (k+1)(k+2)(k+3) = \text{RHS}$
- QED.



**(b) [5 points] For all integers  $n \geq 1$ ,  $n(n^2 + 5)$  is a multiple of 6.**

- Proof.
  - Let  $P(n)$  be the predicate  $6|n(n^2+5)$
  - Base step: We prove  $P(1)$  holds:  $6|6$  is true.
  - Inductive step: We prove for any integer  $k \geq 1$ ,  $P(k) \rightarrow P(k+1)$ 
    - Let  $k$  be an arbitrary integer and  $k \geq 1$ .
    - Assume  $P(k)$  holds. That is  $6|k(k^2+5)$
    - We need to prove  $P(k+1)$ , namely,  $6|(k+1)(k^2+2k+6)$ 
      - $(k+1)(k^2+2k+6) = k^3+3k^2+8k+6 = (k^3+5k)+3(k^2+k+2)$
      - Above is a multiple of 6 because  $6 | (k^3+5k)$  and  $2 | (k^2+k+2)$
- QED.

(c) [5 points] For all integers  $n \geq 0$ ,

$$1 + \frac{2}{3} + \frac{4}{9} + \cdots + \left(\frac{2}{3}\right)^n = 3 \left[ 1 - \left(\frac{2}{3}\right)^{n+1} \right]$$

- Proof.
  - Let  $P(n)$  be the predicate  $1 + (2/3)^1 + \dots + (2/3)^n = 3[1 - (2/3)^{n+1}]$
  - Base step: We prove  $P(0)$  holds: LHS=1, RHS=1
  - Inductive step: We prove for any integer  $k \geq 1$ ,  $P(k) \rightarrow P(k+1)$ 
    - Let  $k$  be an arbitrary integer and  $k \geq 1$ .
    - Assume  $P(k)$  holds. That is  $1 + (2/3)^1 + \dots + (2/3)^k = 3[1 - (2/3)^{k+1}]$
    - We need to prove  $P(k+1)$ , namely,  $1 + (2/3)^1 + \dots + (2/3)^k + (2/3)^{k+1} = 3[1 - (2/3)^{k+2}]$ 
      - LHS=  $3[1 - (2/3)^{k+1}] + (2/3)^{k+1}$  = RHS
- QED.

(d) [5 points] Suppose that  $c_1, c_2, c_3, \dots$  is a sequence defined as follows:

$$c_1 = 3, c_2 = -9$$

$$c_k = 7c_{k-1} - 10c_{k-2} \quad \text{for all integers } k \geq 3$$

Prove that  $c_n = 4 \cdot 2^n - 5^n$  for all integers  $n \geq 1$ .

- Proof.
  - Let  $P(n)$  be the predicate  $c_n = 4 \cdot 2^n - 5^n$
  - Base step: We prove  $P(1)$  and  $P(2)$  hold.
  - Inductive step: We prove for any integer  $k \geq 2$ ,  $P(1), \dots, P(k) \rightarrow P(k+1)$ 
    - Let  $k$  be an arbitrary integer and  $k \geq 2$ .
    - Assume  $P(1), P(2), \dots, P(k)$  hold
    - We need to prove  $P(k+1)$ , namely,  $c_{k+1} = 4 \cdot 2^{k+1} - 5^{k+1}$ 
      - By definition.  $\text{LHS} = 7c_k - 10c_{k-1} = 7(4 \cdot 2^k - 5^k) - 10(4 \cdot 2^{k-1} - 5^{k-1}) = \dots \text{ RHS}$
- QED.